issues/Tmp.fst
@@ -1,0 +1,6 @@
+module Tmp
+open FStar.Seq
+module Seq = FStar.Seq
+let input  = Seq.seq_of_list [3; 1; 2]
+let output = Seq.seq_of_list [1; 2; 3]// Spec: sorted ∧ permutation
+let soundness_test () : Lemma(is_sorted output /\ is_permutation input output)= ()   // F* + Z3 discharge this automatically
